Refactored the ultimate quicksort to make it even more ultimate.

Sorting/QuickSort.v
@@ -13,13 +13,14 @@ Set Implicit Arguments.
 Local Hint Unfold lt.
 Local Hint Resolve le_n_S filter_length.
 
-Function qs (A : LinDec) (l : list A) {measure length l} : list A :=
+(* TODO: remove *)
+(*Function qs (A : LinDec) (l : list A) {measure length l} : list A :=
 match l with
     | [] => []
     | h :: t => qs A (filter (fun x : A => leqb x h) t) ++
            h :: qs A (filter (fun x : A => negb (leqb x h)) t)
 end.
-Proof. all: simpl; auto. Defined.
+Proof. all: simpl; auto. Defined.*)
 
 Local Hint Extern 0 (length _ < length _) =>
 match goal with
@@ -27,15 +28,17 @@ match goal with
         apply filter_lengthOrder
 end.
 
-Function qs2 (A : LinDec) (l : list A) {measure length l} : list A :=
+(* TODO: remove *)
+(*Function qs2 (A : LinDec) (l : list A) {measure length l} : list A :=
 match l with
     | [] => []
     | h :: t =>
         let (lo, hi) := bifilter (fun x : A => x <=? h) t in
         qs2 A lo ++ h :: qs2 A hi
 end.
-Proof. all: auto. Defined.
+Proof. all: auto. Defined.*)
 
+(* TODO: remove *)
 Function hqs (n : nat) (A : LinDec) (sort : list A -> list A) (l : list A)
   {measure length l} : list A :=
   if @leqb natle (length l) n
@@ -47,27 +50,6 @@ Function hqs (n : nat) (A : LinDec) (sort : list A -> list A) (l : list A)
               hqs n A sort lo ++ h :: hqs n A sort hi
   end.
 Proof. all: auto. Defined.
-
-Function ghqs
-  (n : nat) (A : LinDec)
-  (sort : Sort) (*list A -> list A)*) (partition : Partition A)
-  (l : list A) {measure length l} : list A :=
-    if @leqb natle (length l) (S n)
-    then sort A l
-    else match l with
-        | [] => []
-        | h :: t =>
-            let '(lo, eq, hi) := partition h t in
-              ghqs n sort partition lo ++
-              h :: eq ++
-              ghqs n sort partition hi
-    end.
-Proof.
-  intros. apply len_hi in teq1. cbn. omega.
-  intros. apply len_lo in teq1. cbn. omega.
-Defined.
-
-Arguments ghqs _ _ _ _ _ : clear implicits.
 
 (** Time to generalize [ghqs]:
     - Rather that [n], the length of the desired "small list",
@@ -103,16 +85,29 @@ Class Pivot (A : LinDec) : Type :=
 
 Coercion pivot : Pivot >-> Funclass.
 
+Class AdHocSort {A : LinDec} (small : Small A) : Type :=
+{
+    adhoc :> list A -> list A;
+    adhoc_sorted :
+      forall l l' : list A,
+        small l = inl l' -> sorted A (adhoc l');
+    adhoc_perm :
+      forall l l' : list A,
+        small l = inl l' -> perm A l' (adhoc l');
+}.
+
+Coercion adhoc : AdHocSort >-> Funclass.
+
 Function ultimate_qs
   (A : LinDec)
   (small : Small A)
-  (sort : Sort)
+  (adhoc : AdHocSort small)
   (choosePivot : Pivot A)
   (partition : Partition A)
   (l : list A)
   {measure length l} : list A :=
 match small l with
-    | inl l' => sort A l'
+    | inl l' => adhoc l'
     | inr (h, t) =>
         let
           '(pivot, rest) := choosePivot h t
@@ -120,9 +115,9 @@ match small l with
         let
           '(lo, eq, hi) := partition pivot rest
         in
-        ultimate_qs small sort choosePivot partition lo ++
-        pivot :: eq ++
-        ultimate_qs small sort choosePivot partition hi
+          ultimate_qs adhoc choosePivot partition lo ++
+          pivot :: eq ++
+          ultimate_qs adhoc choosePivot partition hi
 end.
 Proof.
   all: intros;
@@ -132,3 +127,105 @@ Proof.
   2: apply len_lo in teq2.
   all: cbn in *; omega.
 Defined.
+
+(** Ordinary quicksort using [ultimate_qs] *)
+
+Instance head_Small (A : LinDec) : Small A :=
+{
+    small :=
+      fun l : list A =>
+      match l with
+          | [] => inl []
+          | h :: t => inr (h, t)
+      end;
+}.
+Proof.
+  all: destruct l; cbn; inv 1.
+Defined.
+
+Instance head_Pivot (A : LinDec) : Pivot A :=
+{
+    pivot :=
+      fun (h : A) (t : list A) => (h, t)
+}.
+Proof. inv 1. Defined.
+
+Instance bifilter_Partition (A : LinDec) : Partition A :=
+{
+    partition x l :=
+      let '(lo, hi) := bifilter (fun y => y <=? x) l in (lo, [], hi)
+}.
+Proof.
+  all: intros; rewrite bifilter_spec in H; inv H.
+    apply filter_In in H0. firstorder dec.
+    apply filter_In in H0. dec.
+      destruct H0. inv H0.
+      destruct H0. apply LinDec_not_leq_lt in n. firstorder.
+    cbn. omega.
+    cbn. unfold perm. intros. rewrite count_app. apply count_filter.
+Defined.
+
+Instance id_AdHocSort (A : LinDec) : AdHocSort (head_Small A) :=
+{
+    adhoc := id;
+}.
+Proof.
+  all: destruct l; inv 1; constructor.
+Defined.
+
+Instance Partition_filter (A : LinDec) : Partition A :=
+{
+    partition x l :=
+      (filter (fun y => y <=? x) l, [],
+       filter (fun y => negb (y <=? x)) l)
+}.
+Proof.
+  all: intros; inv H.
+    rewrite filter_In in H0. firstorder dec.
+    rewrite filter_In in H0. dec.
+      destruct H0. inv H0.
+      destruct H0. apply LinDec_not_leq_lt in n. firstorder.
+    cbn. omega.
+    cbn. unfold perm. intros. rewrite count_app. apply count_filter.
+Defined.
+
+Definition qs A :=
+  ultimate_qs (id_AdHocSort A) (head_Pivot A) (Partition_filter A).
+
+Definition qs2 A :=
+  ultimate_qs (id_AdHocSort A) (head_Pivot A) (bifilter_Partition A).
+
+Compute qs2 natle [4; 3; 2; 1].
+
+(** Like [ultimate_qs], but additionally has knowledge about the
+    recursion's depth. *)
+
+(*Function ultimate_qs
+  (A : LinDec)
+  (small : Small A)
+  (adhoc : AdHocSort small)
+  (choosePivot : Pivot A)
+  (partition : Partition A)
+  (l : list A)
+  {measure length l} : list A :=
+match small l with
+    | inl l' => adhoc l'
+    | inr (h, t) =>
+        let
+          '(pivot, rest) := choosePivot h t
+        in
+        let
+          '(lo, eq, hi) := partition pivot rest
+        in
+          ultimate_qs adhoc choosePivot partition lo ++
+          pivot :: eq ++
+          ultimate_qs adhoc choosePivot partition hi
+end.
+Proof.
+  all: intros;
+    apply small_inr, Permutation_length in teq;
+    apply pivot_spec, Permutation_length in teq1.
+  1: apply len_hi in teq2.
+  2: apply len_lo in teq2.
+  all: cbn in *; omega.
+Defined.*)
